theories/SemiPreOrder.v
@@ -1,0 +1,108 @@
+(***
+ *** Semi Pre-Orders
+ ***)
+
+Require Export Coq.Program.Tactics.
+Require Export Coq.Setoids.Setoid.
+Require Export Coq.Classes.Morphisms.
+Require Export Coq.Arith.Arith_base.
+Require Export Coq.Relations.Relations.
+Require Export Coq.Classes.RelationClasses.
+
+
+Section SemiPreOrder.
+
+Context {A:Type}.
+
+(* Semi-reflexivity: reflexivity on the field of the relation *)
+Class SemiReflexive (R : relation A) :=
+    semi_reflexivity : forall (x y : A), (R x y \/ R y x) -> R x x.
+
+(* A Semi-PreOrder is a pre-order just on the field of the relation *)
+Class SemiPreOrder (R : relation A) : Prop :=
+  {
+    SemiPreOrder_SemiReflexive :> SemiReflexive R | 2 ;
+    SemiPreOrder_Transitive :> Transitive R | 2
+  }.
+
+(* A PreOrder is always a Semi-PreOrder *)
+Global Instance PreOrder_SemiPreOrder {R} `{@PreOrder A R} : SemiPreOrder R.
+destruct H; constructor; [ | assumption ].
+intros x y H1; reflexivity.
+Qed.
+
+(* A PER is always a Semi-PreOrder *)
+Global Instance PER_SemiPreOrder {R} `{@PER A R} : SemiPreOrder R.
+destruct H; constructor; [ | assumption ].
+intros x y H1; destruct H1; transitivity y;
+  try assumption; symmetry; assumption.
+Qed.
+
+(* Symmetric closure *)
+Definition clos_sym (R:relation A) : relation A :=
+  fun x y => R x y \/ R y x.
+
+(* The symmetric closure of any relation is symmetric *)
+Global Instance sym_clos_Symmetric {R} : Symmetric (clos_sym R).
+intros x y H; destruct H; [ right | left ]; assumption.
+Qed.
+
+(* Symmetric-Transitive closure *)
+Inductive clos_sym_trans (R:relation A) (x:A) : A -> Prop :=
+| st_step (y:A) : R x y -> clos_sym_trans R x y
+| st_rstep (y:A) : R y x -> clos_sym_trans R x y
+| st_trans (y z:A) : clos_sym_trans R x y -> clos_sym_trans R y z -> clos_sym_trans R x z.
+
+(* The symmetric-transitive closure of a SemiPreOrder is a PER *)
+Global Instance SemiPreOrder_sym_clos {R} `{@SemiPreOrder R} : PER (clos_sym_trans R).
+destruct H; constructor.
++ intros x y Rxy. induction Rxy.
+  - apply st_rstep; assumption.
+  - apply st_step; assumption.
+  - apply (st_trans _ _ y); assumption.
++ intros x y z Rxy Ryz. apply (st_trans _ _ y); assumption.
+Qed.
+
+End SemiPreOrder.
+
+
+(***
+ *** So-Called Logical Relations
+ ***)
+
+(* A "logical relation" is just a distinguished semi-preorder on a type *)
+Class LR_Op (A:Type) : Type := lr_leq : relation A.
+
+(* To be valid, a logical relation must actually be a semi-preorder *)
+Class LR A `{R:LR_Op A} : Prop :=
+  { lr_SemiPreOrder :> @SemiPreOrder A lr_leq }.
+
+Notation "x '<~' y" := (lr_leq x y) (at level 80, no associativity).
+
+(* Helper notation for using the PER associated with a logical relation *)
+Definition lr_eq `{LR_Op} : relation A := clos_sym_trans lr_leq.
+
+Notation "x '~~' y" := (lr_eq x y) (at level 80, no associativity).
+
+Instance le_eq_SemiPreOrder `{LR} : SemiPreOrder lr_eq.
+Proof. apply PER_SemiPreOrder. Qed.
+
+
+(***
+ *** Pre-Defined Logical Relations
+ ***)
+
+(* The logical relation for pairs is just the pointwise relation *)
+Instance LR_Op_pair {A B} `{LR_Op A} `{LR_Op B} : LR_Op (A * B) :=
+  fun p1 p2 =>
+    lr_leq (fst p1) (fst p2) /\ lr_leq (snd p1) (snd p2).
+
+Instance LR_pair {A B} `{LR A} `{LR B} : LR (A * B).
+Proof.
+  constructor; constructor.
+  intros p1 p2 R12; split; destruct R12; destruct H1;
+    first [ apply (semi_reflexivity _ (fst p2)) | apply (semi_reflexivity _ (snd p2)) ];
+    first [ left; assumption | right; assumption ].
+  intros p1 p2 p3 R12 R23; destruct R12; destruct R23; split;
+    [ transitivity (fst p2) | transitivity (snd p2) ]; assumption.
+Qed.
